some progress towards Dyckhoff & Negri Lemma 4.2

ljt/ljt_dn.v
@@ -171,21 +171,137 @@ eapply (rr_ext_relI_eqc _ _ _ [] _).
 apply ImpRinv_I. reflexivity. clear r.
 apply LJA_der_id. apply AccT_dnsubfml. Qed.
 
-(* Lemma 4.1 of Dyckhoff & Negri JSL 2000
+(* Lemma 4.1 of Dyckhoff & Negri JSL 2000 *)
+(* relevant property of sequent to be proved by induction *)
+Definition l41prop {V} (D : PropF V) seq := 
+  forall G1 G2, seq = (G1 ++ G2, D) -> 
+  forall B E, derrec LJArules emptyT (fmlsext G1 G2 [B], E) ->
+  derrec LJArules emptyT (apfst (fmlsext G1 G2) ([Imp D B], E)).
 
-Check gstep.gen_step_lemT.
+(*
+
+Check gen_step_lemT.
 Check gen_step_c_lem.  Check gen_step_tr_lem. Check gf2_step_tr_lem.
 Check height_step_tr_lem.
 
+(* proof using gen_step_lemT *)
+Definition l41dtprop {V} rules prems (D : PropF V) dt := 
+  l41prop D (@derrec_fc_concl _ rules prems dt).
 
-Lemma LJA_ImpL_adm V G1 G2 B D E : adm LJArules 
-  (map (apfst (fmlsext G1 G2)) [ ([], D) ; ([B], E)])
-  ((apfst (fmlsext G1 G2)) ([@Imp V D B], E)).
-Proof. apply admI. intro drs.
-inversion drs. subst. clear drs.
-apply dersrec_singleD in X0.
-revert X0.  revert E. revert B.
 
+Lemma LJA_ImpL_adm V D : forall dt,
+  @l41dtprop V LJArules emptyT D dt.
+Proof. intro.
+eapply height_step_tr_lem.
+admit.
+clear dt.
+intros. 
+unfold height_step_tr.
+unfold gf2_step_tr.
+intros sub fdt.
+unfold l41dtprop.
+unfold l41prop.
+
+  
+  
+Lemma LJA_ImpL_adm V D : forall seq, derrec LJArules emptyT seq -> 
+  @l41prop V D seq.
+Proof. eapply gen_step_lemT.
+admit.
+intros * ljpc.
+unfold gen_step.
+intros acc fdl der.
+unfold l41prop.
+intros * cgg * dbe.
+destruct ljpc.
+inversion r. clear r. subst. destruct X.
+- admit.
+- 
+
+Lemma LJA_inv_ail V G1 G2 E ps c :
+  (@LJAilrules V) ps c ->
+  derrec LJArules emptyT (G1 ++ c ++ G2, E) -> 
+  dersrec LJArules emptyT (map (apfst (fmlsext G1 G2)) 
+  (map (flip pair E) ps)).
+Proof. intros ljpc dce.  destruct ljpc ; destruct i.
+- apply LJA_can_rel_ImpL_And_inv in dce.
+unfold can_rel in dce.
+apply dersrec_singleI.
+apply dce.  simpl.  unfold fmlsext.
+eapply srs_ext_relI_eq.  apply fslr_I.
+apply ImpL_And_invs_I.  reflexivity.  reflexivity.
+- apply LJA_can_rel_ImpL_Or_inv in dce.
+unfold can_rel in dce.
+apply dersrec_singleI.
+apply dce.  simpl.  unfold fmlsext.
+eapply srs_ext_relI_eq.  apply fslr_I.
+apply ImpL_Or_invs_I.  reflexivity.  reflexivity. Qed.
+
+Lemma LJAil_psne V ps c : (@LJAilrules V) ps c ->
+  sigT (fun p => sigT (fun pt => ps = p :: pt)).
+Proof. intro ljpc. 
+destruct ljpc ; destruct i ; eexists ; eexists ; reflexivity. Qed.
+
+Lemma hs_LJA_ImpL_adm V (D : PropF V)
+  c (dt : derrec LJArules emptyT c) ps (br : botRule_fc (fcI dt) ps c) :
+  @LJArules V ps c -> 
+  height_step_tr (dtfun l41prop) D isubfml (fcI dt).
+Proof. intro ljpc. inversion ljpc ; subst ; clear ljpc.
+inversion X ; subst ; clear X.
+destruct X0.
+- (* left compound Imp rules, invertible *)
+apply (gs_hs br).
+
+need to make this a separate lemma 
+
+unfold gen_step. intros sad fp dc. clear sad br.
+unfold l41prop. intros * ceq * dbe.
+inversion r. subst. clear r. 
+rewrite ceq in dc.
+simpl in ceq. unfold fmlsext in ceq.
+inversion ceq. subst. clear ceq.
+acacD'T2 ; subst.
++
+(* apply rule in desired conclusion *)
+simpl.  unfold fmlsext.  assoc_mid c0.
+eapply derI.  eapply fextI.  eapply rmI_eqc.
+eapply il_anc.  apply rmI.  apply H. reflexivity.
+apply dersrecI_forall.  intros c cin.
+apply InT_mapE in cin. cD.  apply InT_mapE in cin1. cD.
+(* invert rule in dbe *)
+revert dbe. unfold fmlsext. assoc_mid c0. intro dbe.
+pose (LJA_inv_ail _ _ H dbe).
+eapply dersrecD_forall in d. 
+2: apply InT_map.  2: apply InT_map. 2: eassumption.
+eapply ForallTD_forall in fp.
+2: apply InT_map.  2: apply InT_map. 2: eassumption.
+unfold l41prop in fp.
+inversion cin3. inversion cin0. subst. clear cin3 cin0.
+unfold fmlsext.  assoc_single_mid.
+simpl in fp.  unfold fmlsext in fp.
+apply (snd fp). list_eq_assoc.
+simpl in d.  unfold fmlsext in d.
+apply (eq_rect _ _ d). list_eq_assoc.
+
+
+
+
+
+Lemma LJA_ImpL_adm V D : forall seq, derrec LJArules emptyT seq -> 
+  @l41prop V D seq.
+Proof.  intros seq dt.
+assert (dtfun l41prop D (fcI dt)).
+all: cycle 1.
+unfold dtfun in X. simpl in X.  rewrite !der_concl_eq in X. exact X.
+apply (height_step_tr_lem _ (AccT_isubfml D)).
+intros. clear seq dt.  destruct dt0.
+apply (hs_LJA_ImpL_adm (get_botrule _) (bot_is_rule _)).  Qed.
+  
+
+    A isubfml (fcI dl) (fcI dr).
+Proof. intros ma mb. inversion mb ; subst.
+- inversion ma ; subst.
+apply (gs2_hs2 brl brr).
 
 
 *)
